open import net.cruhland.axioms.Eq as Eq using (_≃_)
open Eq.≃-Reasoning
open import net.cruhland.axioms.Sets.Base using (SetAxioms)
open import net.cruhland.axioms.Sets.Complement using (Complement)
open import net.cruhland.axioms.Sets.Difference using (Difference)
open import net.cruhland.axioms.Sets.Empty using (EmptySet)
open import net.cruhland.axioms.Sets.Intersection using (PairwiseIntersection)
open import net.cruhland.axioms.Sets.Pair using (PairSet)
open import net.cruhland.axioms.Sets.Singleton using (SingletonSet)
import net.cruhland.axioms.Sets.Subset as Subset
open import net.cruhland.axioms.Sets.Union using (PairwiseUnion)
open import net.cruhland.models.Function using (_∘_; flip)
open import net.cruhland.models.Logic
  using (_∧_; ∧-intro; ∨-introᴸ; ∨-introᴿ; ∨-map; ∨-rec; _↯_)
open import net.cruhland.models.Setoid using (El; Setoid₀)

module net.cruhland.axioms.Sets.Properties
    (SA : SetAxioms)
    (CM : Complement SA)
    (ES : EmptySet SA)
    (PI : PairwiseIntersection SA)
    (PS : PairSet SA)
    (PU : PairwiseUnion SA ES)
    (SD : Difference SA)
    (SS : SingletonSet SA)
    where
  open Complement CM using (∁; x∈∁A-elim; x∈∁A-intro)
  open Difference SD using (_∖_; x∈A∖B-elim; x∈A∖B-elimᴸ; x∈A∖B-intro)
  open EmptySet ES using (∅; x∉∅)
  open PairSet PS using (pair; x∈pab-elimᴿ; x∈pab-introᴸ; x∈pab-introᴿ)
  open PairwiseIntersection PI
    using ( _∩_; ∩-comm; x∈A∩B-elim; x∈A∩B-elimᴸ; x∈A∩B-elimᴿ; x∈A∩B-intro₂
          ; ∩-substᴸ; ∩-substᴿ)
  open PairwiseUnion PU
    using ( _∪_; ∪-comm; x∈A∪B-elim; x∈A∪B-intro; x∈A∪B-introᴸ; x∈A∪B-introᴿ
          ; ∪-substᴸ; ∪-substᴿ)
  open SetAxioms SA using (_∈_; PSet₀)
  open SingletonSet SS using (singleton; x∈sa-elim; x∈sa-intro)
  open Subset SA using (_⊆_; ⊆-antisym; ⊆-intro)
  import net.cruhland.axioms.Sets.Equality SA as SE

  private
    variable
      S : Setoid₀
      A B C : PSet₀ S

  ∅-⊆ : ∅ ⊆ A
  ∅-⊆ = ⊆-intro (_↯ x∉∅)

  A⊆∅→A≃∅ : A ⊆ ∅ → A ≃ ∅
  A⊆∅→A≃∅ A⊆∅ = ⊆-antisym A⊆∅ ∅-⊆

  ∪⊆-elimᴸ : A ∪ B ⊆ C → A ⊆ C
  ∪⊆-elimᴸ (⊆-intro x∈A∪B→x∈C) = ⊆-intro (x∈A∪B→x∈C ∘ x∈A∪B-introᴸ)

  ∪⊆-elimᴿ : A ∪ B ⊆ C → B ⊆ C
  ∪⊆-elimᴿ (⊆-intro x∈A∪B→x∈C) = ⊆-intro (x∈A∪B→x∈C ∘ x∈A∪B-introᴿ)

  ∪⊆-elim : A ∪ B ⊆ C → A ⊆ C ∧ B ⊆ C
  ∪⊆-elim A∪B⊆C = ∧-intro (∪⊆-elimᴸ A∪B⊆C) (∪⊆-elimᴿ A∪B⊆C)

  ⊆∪-introᴸ : A ⊆ A ∪ B
  ⊆∪-introᴸ = ⊆-intro x∈A∪B-introᴸ

  ⊆∪-introᴿ : B ⊆ A ∪ B
  ⊆∪-introᴿ = ⊆-intro x∈A∪B-introᴿ

  ∪⊆-intro₂ : A ⊆ C → B ⊆ C → A ∪ B ⊆ C
  ∪⊆-intro₂ (⊆-intro x∈A→x∈C) (⊆-intro x∈B→x∈C) =
    ⊆-intro (∨-rec x∈A→x∈C x∈B→x∈C ∘ x∈A∪B-elim)

  pab≃sa∪sb : {a b : El S} → pair a b ≃ singleton {S = S} a ∪ singleton b
  pab≃sa∪sb {S = S} {a} {b} = ⊆-antisym (⊆-intro forward) (⊆-intro backward)
    where
      forward : ∀ {x} → x ∈ pair a b → x ∈ singleton a ∪ singleton b
      forward x∈pab with x∈pab-elimᴿ x∈pab
      ... | ∨-introᴸ x≈a = x∈A∪B-introᴸ (x∈sa-intro x≈a)
      ... | ∨-introᴿ x≈b = x∈A∪B-introᴿ (x∈sa-intro x≈b)

      backward : ∀ {x} → x ∈ singleton a ∪ singleton b → x ∈ pair a b
      backward x∈sa∪sb with x∈A∪B-elim x∈sa∪sb
      ... | ∨-introᴸ x∈sa = x∈pab-introᴸ (x∈sa-elim x∈sa)
      ... | ∨-introᴿ x∈sb = x∈pab-introᴿ (x∈sa-elim x∈sb)

  ∩-∅ᴸ : ∅ ∩ A ≃ ∅
  ∩-∅ᴸ = A⊆∅→A≃∅ (⊆-intro x∈A∩B-elimᴸ)

  ∩-∅ᴿ : A ∩ ∅ ≃ ∅
  ∩-∅ᴿ = Eq.trans ∩-comm ∩-∅ᴸ

  ∩⊆-introᴸ : A ∩ B ⊆ A
  ∩⊆-introᴸ = ⊆-intro x∈A∩B-elimᴸ

  ∩⊆-introᴿ : A ∩ B ⊆ B
  ∩⊆-introᴿ = ⊆-intro x∈A∩B-elimᴿ

  ⊆∩-intro₂ : C ⊆ A → C ⊆ B → C ⊆ A ∩ B
  ⊆∩-intro₂ (⊆-intro x∈C→x∈A) (⊆-intro x∈C→x∈B) =
    ⊆-intro λ x∈C → x∈A∩B-intro₂ (x∈C→x∈A x∈C) (x∈C→x∈B x∈C)

  ⊆∩-elimᴸ : C ⊆ A ∩ B → C ⊆ A
  ⊆∩-elimᴸ (⊆-intro x∈C→x∈A∩B) = ⊆-intro (x∈A∩B-elimᴸ ∘ x∈C→x∈A∩B)

  ⊆∩-elimᴿ : C ⊆ A ∩ B → C ⊆ B
  ⊆∩-elimᴿ (⊆-intro x∈C→x∈A∩B) = ⊆-intro (x∈A∩B-elimᴿ ∘ x∈C→x∈A∩B)

  ⊆∩-elim : C ⊆ A ∩ B → C ⊆ A ∧ C ⊆ B
  ⊆∩-elim C⊆A∩B = ∧-intro (⊆∩-elimᴸ C⊆A∩B) (⊆∩-elimᴿ C⊆A∩B)

  ∩-preserves-⊆ᴸ : A ⊆ B → C ∩ A ⊆ C ∩ B
  ∩-preserves-⊆ᴸ {A = A} {B} {C} (⊆-intro x∈A→x∈B) = ⊆-intro x∈C∩A→x∈C∩B
    where
      x∈C∩A→x∈C∩B : ∀ {x} → x ∈ C ∩ A → x ∈ C ∩ B
      x∈C∩A→x∈C∩B x∈C∩A =
        let ∧-intro x∈C x∈A = x∈A∩B-elim x∈C∩A
         in x∈A∩B-intro₂ x∈C (x∈A→x∈B x∈A)

  ∩-over-∪ᴿ : (A ∪ B) ∩ C ≃ A ∩ C ∪ B ∩ C
  ∩-over-∪ᴿ {A = A} {B} {C} = ⊆-antisym (⊆-intro forward) (⊆-intro backward)
    where
      forward : ∀ {x} → x ∈ (A ∪ B) ∩ C → x ∈ A ∩ C ∪ B ∩ C
      forward x∈[A∪B]∩C =
        let ∧-intro x∈A∪B x∈C = x∈A∩B-elim x∈[A∪B]∩C
            x∈A∨x∈B = x∈A∪B-elim x∈A∪B
            x∈A∩C∨x∈B∩C =
              ∨-map (flip x∈A∩B-intro₂ x∈C) (flip x∈A∩B-intro₂ x∈C) x∈A∨x∈B
         in x∈A∪B-intro x∈A∩C∨x∈B∩C

      backward : ∀ {x} → x ∈ A ∩ C ∪ B ∩ C → x ∈ (A ∪ B) ∩ C
      backward x∈A∩C∪B∩C with x∈A∪B-elim x∈A∩C∪B∩C
      ... | ∨-introᴸ x∈A∩C =
        let ∧-intro x∈A x∈C = x∈A∩B-elim x∈A∩C
         in x∈A∩B-intro₂ (x∈A∪B-introᴸ x∈A) x∈C
      ... | ∨-introᴿ x∈B∩C =
        let ∧-intro x∈B x∈C = x∈A∩B-elim x∈B∩C
         in x∈A∩B-intro₂ (x∈A∪B-introᴿ x∈B) x∈C

  ∩-over-∪ᴸ : A ∩ (B ∪ C) ≃ A ∩ B ∪ A ∩ C
  ∩-over-∪ᴸ {A = A} {B} {C} =
    begin
      A ∩ (B ∪ C)
    ≃⟨ ∩-comm ⟩
      (B ∪ C) ∩ A
    ≃⟨ ∩-over-∪ᴿ ⟩
      B ∩ A ∪ C ∩ A
    ≃⟨ ∪-substᴸ ∩-comm ⟩
      A ∩ B ∪ C ∩ A
    ≃⟨ ∪-substᴿ ∩-comm ⟩
      A ∩ B ∪ A ∩ C
    ∎

  ∪-over-∩ᴸ : A ∪ (B ∩ C) ≃ (A ∪ B) ∩ (A ∪ C)
  ∪-over-∩ᴸ {A = A} {B} {C} = ⊆-antisym (⊆-intro forward) (⊆-intro backward)
    where
      forward : ∀ {x} → x ∈ A ∪ (B ∩ C) → x ∈ (A ∪ B) ∩ (A ∪ C)
      forward x∈A∪[B∩C] with x∈A∪B-elim x∈A∪[B∩C]
      ... | ∨-introᴸ x∈A = x∈A∩B-intro₂ (x∈A∪B-introᴸ x∈A) (x∈A∪B-introᴸ x∈A)
      ... | ∨-introᴿ x∈B∩C =
        let ∧-intro x∈B x∈C = x∈A∩B-elim x∈B∩C
         in x∈A∩B-intro₂ (x∈A∪B-introᴿ x∈B) (x∈A∪B-introᴿ x∈C)

      backward : ∀ {x} → x ∈ (A ∪ B) ∩ (A ∪ C) → x ∈ A ∪ (B ∩ C)
      backward x∈[A∪B]∩[A∪C] with x∈A∪B-elim x∈A∪B | x∈A∪B-elim x∈A∪C
        where
          x∈A∪B = x∈A∩B-elimᴸ x∈[A∪B]∩[A∪C]
          x∈A∪C = x∈A∩B-elimᴿ x∈[A∪B]∩[A∪C]
      ... | ∨-introᴸ x∈A | ac = x∈A∪B-introᴸ x∈A
      ... | ∨-introᴿ x∈B | ∨-introᴸ x∈A = x∈A∪B-introᴸ x∈A
      ... | ∨-introᴿ x∈B | ∨-introᴿ x∈C = x∈A∪B-introᴿ (x∈A∩B-intro₂ x∈B x∈C)

  ∪-over-∩ᴿ : (A ∩ B) ∪ C ≃ (A ∪ C) ∩ (B ∪ C)
  ∪-over-∩ᴿ {A = A} {B} {C} =
    begin
      (A ∩ B) ∪ C
    ≃⟨ ∪-comm ⟩
      C ∪ (A ∩ B)
    ≃⟨ ∪-over-∩ᴸ ⟩
      (C ∪ A) ∩ (C ∪ B)
    ≃⟨ ∩-substᴸ ∪-comm ⟩
      (A ∪ C) ∩ (C ∪ B)
    ≃⟨ ∩-substᴿ ∪-comm ⟩
      (A ∪ C) ∩ (B ∪ C)
    ∎

  A∖B≃A∩∁B : A ∖ B ≃ A ∩ ∁ B
  A∖B≃A∩∁B {A = A} {B} = ⊆-antisym (⊆-intro forward) (⊆-intro backward)
    where
      forward : ∀ {x} → x ∈ A ∖ B → x ∈ A ∩ ∁ B
      forward x∈A∖B =
        let ∧-intro x∈A x∉B = x∈A∖B-elim x∈A∖B
         in x∈A∩B-intro₂ x∈A (x∈∁A-intro x∉B)

      backward : ∀ {x} → x ∈ A ∩ ∁ B → x ∈ A ∖ B
      backward x∈A∩∁B =
        let ∧-intro x∈A x∈∁B = x∈A∩B-elim x∈A∩∁B
         in x∈A∖B-intro (∧-intro x∈A (x∈∁A-elim x∈∁B))

  A∖B⊆A : A ∖ B ⊆ A
  A∖B⊆A = ⊆-intro x∈A∖B-elimᴸ
